# Limit Rules

see [Classical Math Notation](Classical%20Math%20Notation%20eb53679093ce497baa118d7bfde14d6c.md), [Math Notation](Math%20Notation%207bc4575af1e541d6946b955774161a6a.md)

## General Rules

- $\lim_{x \to \infty} 1 / (x ^ r) = 0\ if\ r > 0$
- $\lim_{x \to 0} 1 / x = \infty$
- $\lim_{x \to a} \ne \varnothing\ \equiv\ \lim_{x \to a^+} = \lim_{x \to a^-} \ne \varnothing$

## Arithmetic Rules

let $c$ be a constant and ensure $\lim_{x \to a}f(x)$ and $\lim_{x \to a}g(x)$ are [Limit that Exists](Limit%20that%20Exists%206a9c8aa5e455457ba848eb37d8d12bc7.md) 

- $\lim_{x \to a}[f(x) + g(x)] = \lim_{x \to a}f(x) + \lim_{x \to a}g(x)$
- $\lim_{x \to a}[f(x) - g(x)] = \lim_{x \to a}f(x) - \lim_{x \to a}g(x)$
- $\lim_{x \to a}[c f(x)] = c\lim_{x \to a}f(x)$
- $\lim_{x \to a}[f(x) g(x)] = \lim_{x \to a}f(x) \times \lim_{x \to a}g(x)$
- $\lim_{x \to a}\frac{f(x)}{g(x)} = \frac{\lim_{x \to a}f(x)}{\lim_{x \to a}g(x)}$ if $\lim_{x \to a} g(x) \ne 0$
- $\lim_{x \to a}[f(x)]^n = [\lim_{x \to a} f(x)]^n$
- $\lim_{x \to a}\sqrt[n]{f(x)} = \sqrt[n]{\lim_{x \to a} f(x)}$. When $n\ \%\ 2 = 0$, we assume that $\lim_{x \to a} f(x) \ne 0$