# Deriving the Quadratic Formula

see [[classical-math-notation]], [[quadratic-formula]]

$y = a(x - h)^2 + k$

$y = ax^2 + bx + c$

$x = \sqrt{(y - k) / a} + h$

$h = -b / (2a)$ (still to be proven)

$k = f(h)$

$x = \sqrt{(0 - (a(-b / 2a)^2 + b(-b / (2a)) + c)) / a} - b / 2a$

$x = (2a\sqrt{(-(a(-b / 2a)^2 + b(-b / (2a)) + c)) / a} - b) / 2a$

$x = (\sqrt{(-(a(-b / 2a)^2 + b(-b / (2a)) + c)) * 4a} - b) / 2a$

$x = (\sqrt{((ab^2 / 4a^2 - b^2 / (2a)) - c) * 4a} - b) / 2a$

$x = (\sqrt{((b^2 / 4a - 2b^2 / (4a)) - c) * 4a} - b) / 2a$

$x = (\sqrt{((b^2/4a) - c) * 4a} - b) / 2a$

$x = (\sqrt{b^2 - 4ac} - b) / 2a$
