# Hadamard Product

see [[vector]], [[vector-in-rn]], [[matrix]], [[math-notation]]

&mdash; <http://neuralnetworksanddeeplearning.com/chap2.html#the_hadamard_product_$s_\odot_t$>

> **definition**:
>
> let $\mathbb M^{m, n} s \land \mathbb M^{m, n} t$
>
> $(s\ \mathring\mid\ t)^{j, k} = s^{j, k} \mid t^{j, k} \dashv \mathbb N j \land \mathbb N k$, where
>
> - $s\ \mathring\mid\ t$ is the [[hadamard-product]] of the [[matrix]]es $s$ and $t$

> **example**: $\begin{bmatrix} 1 \\\ 2 \end{bmatrix}\ \mathring\mid\ \begin{bmatrix} 3 \\\ 4 \end{bmatrix} = \begin{bmatrix} 1 \mid 3 \\\ 2 \mid 4 \end{bmatrix} = \begin{bmatrix} 3 \\\ 8 \end{bmatrix}$
