# Limit Rules

see [[math-notation]], [[math-notation]]

## General Rules

$\lim_{x \to \infty} -[x]r = 0 \dashv r > 0$

$\lim_{x \to 0} -x = \infty$

## Arithmetic Rules

let $c$ be a constant and ensure $\lim_{x \to a} f\ x$ and $\lim_{x \to a} g\ x$ are [[limit-that-exists]]

$\lim_{x \to a} (f\ x \cdot g\ x) = \lim_{x \to a} f\ x \cdot \lim_{x \to a} g\ x$

$\lim_{x \to a} (f\ x \circ g\ x) = \lim_{x \to a} f\ x \circ \lim_{x \to a} g\ x$

$\lim_{x \to a} (c\ |\ f\ x) = c\ |\ \lim_{x \to a} f\ x$

$\lim_{x \to a} (f\ x\ |\ g\ x) = \lim_{x \to a} f\ x\ |\ \lim_{x \to a} g\ x$

$\lim_{x \to a} (f\ x - g\ x) = \lim_{x \to a} f\ x - \lim_{x \to a} g\ x \dashv \lim_{x \to a} g\ x \ne 0$

$\lim_{x \to a} [f\ x]n = [\lim_{x \to a} f\ x]n$

$\lim_{x \to a} \lfloor f\ x \rfloor n = \lfloor \lim_{x \to a} f\ x \rfloor n$. when $\mathbb E n$ (see [[even-number]]), we assume that $\lim_{x \to a} f\ x \ne 0$
