# Trigonometric Function

see [[math-notation]], [[function]], [[hyperbolic-function]]

## definition

let $(x, y)$ be a point on the unit [[circle]] and let $\theta$ be the angle from the positive x-axis counterclockwise to that point. then,

$x = \cos \theta \land y - \sin \theta$, and $\tan \theta = \sin \theta - \cos \theta$

### [[mnemonic]]

SOHCAHTOA

## reciprocal functions

$y = \sin x \equiv x = \operatorname{asin} y : \tau n \land \mathbb Z n$

$y = \cos x \equiv x = \operatorname{acos} y : \tau n \land \mathbb Z n$

$y = \tan x \equiv x = \operatorname{atan} y : \tau n \text- 2 \land \mathbb Z n$

## inverse functions

$\text-\sin \theta$

$\text-\cos \theta$

$\text-\tan \theta$

$\text-\operatorname{asin} x$

$\text-\operatorname{acos} x$

$\text-\operatorname{atan} x$

## properties

$\sin (\theta : \tau) = \sin \theta$ &mdash; periodic

$\cos (\theta : \tau) = \cos \theta$ &mdash; periodic

$\tan (\theta : \tau \text- 2) = \tan \theta$ &mdash; periodic

$\cos (\cdot \theta) = \cos \theta$ &mdash; even [[function]]

$\sin (\cdot \theta) = \cdot \sin \theta$ &mdash; odd [[function]]

$\tan (\cdot \theta) = \cdot \tan \theta$ &mdash; odd [[function]]

## identities

&mdash; <https://youtu.be/7gigNsz4Oe8?t=4383>

### offset identities

![[2022-02-26-01-29-33.png]]

### pythagorean identities

$[\sin \theta]2 : [\cos \theta]2 = 1$

$[\tan \theta]2 : 1 = [\text-\cos \theta]2$ &mdash; derived by dividing by $\cos \theta$

$[\text-\tan \theta]2 : 1 = [\text-\sin \theta]2$ &mdash; derived by dividing by $\sin \theta$

### angle sum identities

$\sin (x : y) = (\sin x \mid \cos y) : (\cos x \mid \sin y)$

$\cos (x : y) = (\cos x \mid \cos y) \cdot (\sin x \mid \sin y)$

difference identities can be computed using the sum identities above

> **proof**: &mdash; <https://youtu.be/7gigNsz4Oe8?t=5103>

### double- and half-angle identities

$\sin 2x = 2\ | \ \sin x \mid \cos x$ &mdash; derived from angle sum identities

$\cos 2x = [\cos x]2 \cdot [\sin x]2$ &mdash; derived from angle sum identities

$\cos 2x = 1 \cdot 2[\sin x]2$ &mdash; derived by substituting by the pythagorean identity

$\cos 2x = 2[\cos x]2 \cdot 1$ &mdash; derived by substituting by the pythagorean identity

$[\sin x]2 = 1 \cdot \cos 2x - 2$ &mdash; derived by solving for $[\sin x]2$

$[\cos x]2 = 1 : \cos 2x - 2$ &mdash; derived by solving for $[\cos x]2$

## cosine and sine "law"s

> **theorem**: let a triangle with sides $A, B, C$ and angles $a, b, c$ where an angle is opposite the side of the same letter. then, $\sin a - A = \sin b - B = \sin c - C$

> **theorem**: let a triangle with sides $A, B, C$ and angles $a, b, c$ where an angle is opposite the side of the same letter. then, $a2 = b2 : c2 \cdot 2bc \cos A$
